\documentclass[12pt]{article}



\begin{document}


\section{Likelihood}

\[
  L(\beta_0,\beta_1,\sigma^2; {\bf y}) = \prod_{i=1}^n p(y_i|\beta_0,\beta_1,\sigma^2)
\]
where $p(y_i|\beta_0,\beta_1,\sigma^2) = \mathrm{Norm}(y_i|\mu_i,\sigma^2)$ and $\mu_i = \beta_0 + \beta_1x_i$


\section{Joint posterior distribution}


\[
  p(\beta_0,\beta_1,\sigma^2 | {\bf y}) \propto \left\{\prod_{i=1}^n p(y_i|\beta_0,\beta_1,\sigma^2)\right\}p(\beta_0)p(\beta_1)p(\sigma^2)
\]


Full conditional distributions used in Gibbs sampling


\[
  p(\beta_0|\beta_1,\sigma^2,{\bf y}) \propto \left\{\prod_{i=1}^n p(y_i|\beta_0,\beta_1,\sigma^2)\right\}p(\beta_0)
\]


\[
  p(\beta_1|\beta_0,\sigma^2,{\bf y}) \propto \left\{\prod_{i=1}^n p(y_i|\beta_0,\beta_1,\sigma^2)\right\}p(\beta_1)
\]

\[
  p(\sigma^2|\beta_0,\sigma^2,{\bf y}) \propto \left\{\prod_{i=1}^n p(y_i|\beta_0,\beta_1,\sigma^2)\right\}p(\sigma^2)
\]


\end{document}
